Proved most branches for correctness

Regex/NFA/Transition.lean
@@ -1,122 +1,295 @@
 import Regex.Lemmas
 import Regex.NFA.Basic
+import Regex.NFA.Compile
 
 import Mathlib.Data.Set.Basic
+import Mathlib.Data.Set.Lattice
 
 open Set
 
-namespace NFA.Transition
+-- TODO: we may want to prove that all indices are in bounds get rid of Option helpers.
+def Option.charStep : Option NFA.Node → Char → Set Nat
+  | some n, c => n.charStep c
+  | none, _ => ∅
 
-def charStep (nodes : Array Node) (c : Char) (i : Nat) : Set Nat :=
-  if h : i < nodes.size then
-    match nodes[i] with
-    | .char c' next => if c = c' then {next} else ∅
-    | _ => ∅
-  else
-    ∅
+def Option.εStep : Option NFA.Node → Set Nat
+  | some n => n.εStep
+  | none => ∅
 
-def εStep (nodes : Array Node) (i : Nat) : Set Nat :=
-  if h : i < nodes.size then
-    match nodes[i] with
-    | .epsilon next => {next}
-    | .split next₁ next₂ => {next₁, next₂}
-    | _ => ∅
-  else
-    ∅
+namespace NFA
 
-inductive εClosure (nodes : Array Node) : Nat → Set Nat where
-  | base : εClosure nodes i i
-  | step {i j k : Nat} (head : j ∈ εStep nodes i) (tail : εClosure nodes j k) : εClosure nodes i j
+def Option.charStep.simp {nfa : NFA} {i : Nat} {c : Char} :
+  nfa[i]?.charStep c = if h : i < nfa.nodes.size then nfa[i].charStep c else ∅ := by
+  simp [Option.charStep, getElem?]
+  cases Nat.decLt i nfa.nodes.size <;> simp [*]
 
-def εClosureSet (nodes : Array Node) (S : Set Nat) : Set Nat
-  | j => ∃ i ∈ S, j ∈ εClosure nodes i
+theorem Option.charStep.subset_of_le {nfa₁ nfa₂ : NFA} {i : Nat} (le : nfa₁ ≤ nfa₂) :
+  nfa₁[i]?.charStep c ⊆ nfa₂[i]?.charStep c := by
+  simp [Option.charStep.simp]
+  cases Nat.decLt i nfa₁.nodes.size <;> simp [*]
+  case isTrue h =>
+    let ⟨h', le⟩ := le i h
+    simp [h']
+    exact le.left c
+
+def Option.εStep.simp {nfa : NFA} {i : Nat} :
+  nfa[i]?.εStep = if h : i < nfa.nodes.size then nfa[i].εStep else ∅ := by
+  simp [Option.εStep, getElem?]
+  cases Nat.decLt i nfa.nodes.size <;> simp [*]
+
+theorem Option.εStep.subset_of_le {nfa₁ nfa₂ : NFA} {i : Nat} (le : nfa₁ ≤ nfa₂) :
+  nfa₁[i]?.εStep ⊆ nfa₂[i]?.εStep := by
+  simp [Option.εStep.simp]
+  cases Nat.decLt i nfa₁.nodes.size <;> simp [*]
+  case isTrue h =>
+    let ⟨h', le⟩ := le i h
+    simp [h']
+    exact le.right
+
+inductive NFA.εClosure (nfa : NFA) : Nat → Set Nat where
+  | base : εClosure nfa i i
+  | step {i j k : Nat} (head : j ∈ nfa[i]?.εStep) (tail : nfa.εClosure j k) :
+    εClosure nfa i k
+
+theorem εClosure_of_le {nfa₁ nfa₂ : NFA} (le : nfa₁ ≤ nfa₂) (h : j ∈ nfa₁.εClosure i) :
+  j ∈ nfa₂.εClosure i := by
+  induction h with
+  | base => exact .base
+  | step head _ ih => exact .step (mem_of_subset_of_mem (Option.εStep.subset_of_le le) head) ih
+
+theorem εClosure_trans {nfa : NFA} (h₁ : i₂ ∈ nfa.εClosure i₁) (h₂ : i₃ ∈ nfa.εClosure i₂) :
+  i₃ ∈ nfa.εClosure i₁ := by
+  induction h₁ with
+  | base => exact h₂
+  | step head _ ih => exact .step head (ih h₂)
+
+def NFA.εClosureSet (nfa : NFA) (S : Set Nat) : Set Nat
+  | j => ∃ i ∈ S, j ∈ nfa.εClosure i
 
 @[simp]
-theorem subset_εClosureSet : S ⊆ εClosureSet nodes S := by
+theorem subset_εClosureSet {nfa : NFA} : S ⊆ nfa.εClosureSet S := by
   intro i h
   exists i
   exact ⟨h, .base⟩
 
 @[simp]
-theorem εClosureSet_singleton_base : i ∈ εClosureSet nodes {i} := by
+theorem εClosureSet_singleton_base {nfa : NFA} : i ∈ nfa.εClosureSet {i} := by
   exists i
   exact ⟨mem_singleton _, .base⟩
 
 @[simp]
-theorem εClosureSet_singleton_step {i j : Nat} (h : j ∈ εStep nodes i) : j ∈ εClosureSet nodes {i} := by
+theorem εClosureSet_singleton_step {nfa : NFA} {i j : Nat} (h : j ∈ nfa[i]?.εStep) : j ∈ nfa.εClosureSet {i} := by
   exists i
   exact ⟨mem_singleton _, .step h .base⟩
 
 @[simp]
-theorem εClosureSet_empty : εClosureSet nodes ∅ = ∅ := by
+theorem εClosureSet_empty {nfa : NFA} : nfa.εClosureSet ∅ = ∅ := by
   apply eq_empty_of_forall_not_mem
   intro i h
   induction h with
   | intro _ h => apply not_mem_empty _ h.left
 
 @[simp]
-theorem εClosureSet_univ : εClosureSet nodes univ = univ := by
+theorem εClosureSet_univ {nfa : NFA} : nfa.εClosureSet univ = univ := by
   apply eq_univ_of_forall
   intro i
   exists i
   exact ⟨mem_univ _, .base⟩
 
-theorem εClosureSet_monotone : Monotone (εClosureSet nodes) := by
-  intro S₁ S₂ hsub
+theorem εClosureSet_subset {nfa₁ nfa₂ : NFA} (hn : nfa₁ ≤ nfa₂) (hs : S₁ ⊆ S₂) :
+  nfa₁.εClosureSet S₁ ⊆ nfa₂.εClosureSet S₂ := by
   simp [subset_def]
-  intro j hm
-  let ⟨i, h, cls⟩ := hm
-  have hsub' : i ∈ S₂ := mem_of_subset_of_mem hsub h
-  cases cls with
-  | base => exact mem_of_subset_of_mem subset_εClosureSet hsub'
-  | step head tail => exact ⟨i, hsub', .step head tail⟩
-
-def stepSet (nodes : Array Node) (S : Set Nat) (c : Char) : Set Nat
-  | j => ∃ i ∈ S, j ∈ εClosureSet nodes (charStep nodes c i)
+  intro j h
+  let ⟨i, h, cls⟩ := h
+  exact ⟨i, mem_of_subset_of_mem hs h, εClosure_of_le hn cls⟩
 
 @[simp]
-def stepSet_empty : stepSet nodes ∅ c = ∅ := by
-  apply eq_empty_of_forall_not_mem
-  intro i h
-  induction h with
-  | intro _ h => apply not_mem_empty _ h.left
+theorem εClosureSet_idempotent {nfa : NFA} : nfa.εClosureSet (nfa.εClosureSet S) = nfa.εClosureSet S := by
+  apply eq_of_subset_of_subset
+  . simp [subset_def]
+    intro j h
+    let ⟨i, h, cls⟩ := h
+    let ⟨i', h', cls'⟩ := h
+    exact ⟨i', h', εClosure_trans cls' cls⟩
+  . apply subset_εClosureSet
+
+theorem εClosureSet_iUnion_distrib {nfa : NFA} {S : Set α} {f : α → Set Nat} :
+  nfa.εClosureSet (⋃ i ∈ S, f i) = ⋃ i ∈ S, nfa.εClosureSet (f i) := by
+  sorry
+
+def NFA.stepSet (nfa : NFA) (S : Set Nat) (c : Char) : Set Nat :=
+  ⋃ i ∈ S, nfa.εClosureSet (nfa[i]?.charStep c)
 
 @[simp]
-def mem_stepSet_iff : j ∈ stepSet nodes S c ↔ ∃ i ∈ S, j ∈ εClosureSet nodes (charStep nodes c i) := by
-  apply Iff.intro
-  . intro h; exact h
-  . intro h; exact h
+def stepSet_empty {nfa : NFA} : nfa.stepSet ∅ c = ∅ := by
+  simp [NFA.stepSet]
 
-theorem stepSet_monotone (c : Char) : Monotone fun S => stepSet nodes S c := by
-  intro S₁ S₂ h
-  simp [subset_def]
-  intro j i hi hj
-  exact ⟨i, mem_of_subset_of_mem h hi, hj⟩
+-- @[simp]
+-- def mem_stepSet_iff {nfa : NFA} : j ∈ nfa.stepSet S c ↔ ∃ i ∈ S, j ∈ nfa.εClosureSet (nfa[i]?.charStep c) := by
+--   apply Iff.intro
+--   . intro h; exact h
+--   . intro h; exact h
 
-def evalFrom (nodes : Array Node) (S : Set Nat) : List Char → Set Nat :=
-  List.foldl (stepSet nodes) (εClosureSet nodes S)
+@[simp]
+theorem εClosureSet_stepSet {nfa : NFA} :
+  nfa.εClosureSet (nfa.stepSet S c) = nfa.stepSet S c := by
+  apply eq_of_subset_of_subset
+  . conv =>
+      lhs
+      simp [NFA.stepSet, εClosureSet_iUnion_distrib]
+  . exact subset_εClosureSet
 
-theorem evalFrom_monotone :
-  Monotone fun S => evalFrom nodes S cs := by
-  intro S₁ S₂ h
-  simp
-  apply List.foldl_monotone stepSet_monotone cs
-  exact εClosureSet_monotone h
+theorem stepSet_subset {nfa₁ nfa₂ : NFA} (hn : nfa₁ ≤ nfa₂) (hs : S₁ ⊆ S₂) :
+  nfa₁.stepSet S₁ c ⊆ nfa₂.stepSet S₂ c := by
+  simp [subset_def, NFA.stepSet]
+  intro j i h₁ h₂
 
-#check List.foldl_monotone
-#check List.foldl_strictMono
+  exact ⟨
+    i,
+    mem_of_subset_of_mem hs h₁,
+    mem_of_subset_of_mem (εClosureSet_subset hn (Option.charStep.subset_of_le hn)) h₂
+  ⟩
 
-theorem evalFrom_append (eq : s = s₁ ++ s₂) :
-  evalFrom nodes S s = List.foldl (stepSet nodes) (evalFrom nodes S s₁) s₂ := by
+def NFA.evalFrom (nfa : NFA) (S : Set Nat) : List Char → Set Nat :=
+  List.foldl (nfa.stepSet) (nfa.εClosureSet S)
+
+theorem evalFrom_cons {nfa : NFA} :
+  nfa.evalFrom S (c :: cs) = nfa.evalFrom (nfa.stepSet (nfa.εClosureSet S) c) cs := by
+  have h : nfa.stepSet (nfa.εClosureSet S) c = nfa.εClosureSet (nfa.stepSet (nfa.εClosureSet S) c) :=
+    εClosureSet_stepSet.symm
   conv =>
     lhs
-    rw [eq, evalFrom, List.foldl_append]
+    simp [NFA.evalFrom]
+    rw [h]
 
-theorem subset_evalFrom_append (nodes : Array Node) (S : Set Nat) (eq : s = s₁ ++ s₂) :
-  evalFrom nodes S s ⊆ evalFrom nodes (evalFrom nodes S s₁) s₂ := by
-  rw [evalFrom_append eq]
-  apply List.foldl_monotone stepSet_monotone s₂
-  exact subset_εClosureSet
+theorem evalFrom_subset {nfa₁ nfa₂ : NFA} {S₁ S₂ : Set Nat} (hn : nfa₁ ≤ nfa₂) (hs : S₁ ⊆ S₂) :
+  nfa₁.evalFrom S₁ s ⊆ nfa₂.evalFrom S₂ s := by
+  apply le_foldl_of_le
+  . intro _ _ _ hs
+    exact stepSet_subset hn hs
+  . exact εClosureSet_subset hn hs
+
+theorem εClosureSet_evalFrom {nfa : NFA} :
+  nfa.εClosureSet (nfa.evalFrom S s) = nfa.evalFrom S s := by
+  apply eq_of_subset_of_subset
+  . induction s generalizing S with
+    | nil => simp [NFA.evalFrom]; exact le_refl _
+    | cons c cs ih =>
+      rw [evalFrom_cons]
+      exact ih
+  . exact subset_εClosureSet
+
+theorem mem_evalFrom_subset {nfa : NFA} (hmem : next ∈ nfa.evalFrom S₁ s) (hs : S₁ ⊆ nfa.εClosureSet S₂) :
+  next ∈ nfa.evalFrom S₂ s := by
+  apply mem_of_subset_of_mem _ hmem
+  apply le_foldl_of_le
+  . intro _ _ _ hs
+    exact stepSet_subset (le_refl _) hs
+  . suffices nfa.εClosureSet S₁ ⊆ nfa.εClosureSet (nfa.εClosureSet S₂) by
+      simp at this
+      exact this
+    exact εClosureSet_subset (le_refl _) hs
+
+theorem evalFrom_append {nfa : NFA} (eq : s = s₁ ++ s₂) :
+  nfa.evalFrom S s = List.foldl (nfa.stepSet) (nfa.evalFrom S s₁) s₂ := by
+  conv =>
+    lhs
+    rw [eq, NFA.evalFrom, List.foldl_append]
+
+theorem NFA.evalFrom_of_matches (eq : compile.loop r next nfa = nfa')
+  (m : r.matches s) : ∀ nfa'' : NFA, nfa' ≤ nfa'' → next ∈ nfa''.evalFrom {nfa'.val.start.val} s.data := by
+  induction m generalizing next nfa with
+  | @char s c eqs =>
+    intro nfa'' le
+    suffices next ∈ nfa'.val.evalFrom {nfa'.val.start.val} s.data from
+      evalFrom_subset le (le_refl _) this
+    simp [eqs, evalFrom, List.foldl]
+    simp [compile.loop] at eq
+    apply mem_iUnion.mpr
+    exists nfa'.val.start
+    subst eq
+    simp [Option.charStep, Node.charStep]
+  | @epsilon s eqs =>
+    intro nfa'' le
+    suffices next ∈ nfa'.val.evalFrom {nfa'.val.start.val} s.data from
+      evalFrom_subset le (le_refl _) this
+    simp [eqs, evalFrom, List.foldl]
+    simp [compile.loop] at eq
+    exists nfa'.val.start
+    subst eq
+    simp [Option.charStep, Node.charStep]
+    exact εClosure.step (by simp [Option.εStep, Node.εStep]) .base
+  | @alternateLeft s r₁ r₂ m ih =>
+    intro nfa'' le
+    suffices next ∈ nfa'.val.evalFrom {nfa'.val.start.val} s.data from
+      evalFrom_subset le (le_refl _) this
+
+    let nfa₁ := compile.loop r₁ next nfa
+    let start₁ := nfa₁.val.start
+    let nfa₂ := compile.loop r₂ next nfa₁
+    let start₂ := nfa₂.val.start
+    let final := nfa₂.val.addNode (.split start₁ start₂)
+
+    have : nfa'.val = final.val := by
+      simp [eq.symm]
+      rfl
+    rw [this]
+
+    have property : nfa₁.val ≤ final.val :=
+      calc nfa₁.val
+        _ ≤ nfa₂.val := nfa₂.property
+        _ ≤ final.val := final.property
+
+    apply mem_evalFrom_subset (ih rfl final property)
+    simp [Option.εStep, Node.εStep]
+  | @alternateRight s r₁ r₂ m ih =>
+    intro nfa'' le
+    suffices next ∈ nfa'.val.evalFrom {nfa'.val.start.val} s.data from
+      evalFrom_subset le (le_refl _) this
+
+    let nfa₁ := compile.loop r₁ next nfa
+    let start₁ := nfa₁.val.start
+    let nfa₂ := compile.loop r₂ next nfa₁
+    let start₂ := nfa₂.val.start
+    let final := nfa₂.val.addNode (.split start₁ start₂)
+
+    have : nfa'.val = final.val := by
+      simp [eq.symm]
+      rfl
+    rw [this]
+
+    apply mem_evalFrom_subset (ih rfl final final.property)
+    simp [Option.εStep, Node.εStep]
+  | concat s s₁ s₂ r₁ r₂ eqs m₁ m₂ ih₁ ih₂ =>
+    intro nfa'' le
+    suffices next ∈ nfa'.val.evalFrom {nfa'.val.start.val} s.data from
+      evalFrom_subset le (le_refl _) this
+
+    let nfa₂ := compile.loop r₂ next nfa
+    let nfa₁ := compile.loop r₁ nfa₂.val.start nfa₂
+
+    have : nfa'.val = nfa₁.val := by
+      simp [eq.symm]
+      rfl
+    rw [this]
+
+    let ih₁ := ih₁ rfl nfa₁ (le_refl _)
+    let ih₂ := ih₂ rfl nfa₁ nfa₁.property
+
+    apply mem_of_mem_of_subset ih₂
+    show nfa₁.val.evalFrom {nfa₂.val.start.val} s₂.data ⊆ nfa₁.val.evalFrom {nfa₁.val.start.val} s.data
+    rw [evalFrom_append (String.eq_of_append_of_eq_of_append eqs)]
+    apply le_foldl_of_le
+    . intro _ _ _ hs
+      exact stepSet_subset (le_refl _) hs
+    . have : {nfa₂.val.start.val} ⊆ nfa₁.val.evalFrom {nfa₁.val.start.val} s₁.data := by
+        rw [singleton_subset_iff]
+        exact ih₁
+      have : nfa₁.val.εClosureSet {nfa₂.val.start.val} ⊆ nfa₁.val.εClosureSet (nfa₁.val.evalFrom {nfa₁.val.start.val} s₁.data) :=
+        εClosureSet_subset (le_refl _) this
+      rw [εClosureSet_evalFrom] at this
+      exact this
+  | star m ih => sorry
 
 -- theorem evalFrom_of_matches (eq : compileRaw.loop nodes next r = result)
 --   (m : r.matches s) : next ∈ evalFrom result.1 {result.2.val} s.data := by
@@ -168,7 +341,4 @@ theorem subset_evalFrom_append (nodes : Array Node) (S : Set Nat) (eq : s = s₁
 --     sorry
 --   | star => sorry
 
-end NFA.Transition
-
-#check List.foldl_eq_foldr'
-#check List.foldl_monotone
+end NFA
